tests/lean/unfold1.lean
@@ -9,10 +9,10 @@ example (l : list nat) : list.append l [] = l :=
 by do
   get_local `l >>= λ H, induction H [`h, `t, `iH],
   --
-  dunfold [`list.append],
+  dunfold_target [`list.append],
   trace_state,
   trace "------",
   reflexivity,
-  dunfold [`list.append],
+  dunfold_target [`list.append],
   trace_state,
   rewriteH `iH
