tests/lean/unfold_crash.lean
@@ -4,8 +4,8 @@ open nat tactic
 example (a b : nat) : a = succ b → a = b + 1 :=
 by do
   H ← intro `H,
-  try (dunfold_at [`nat.succ] H),
-  dunfold [`add, `has_add.add, `has_one.one, `nat.add, `one],
+  try (dunfold_hyp [`nat.succ] H),
+  dunfold_target [`add, `has_add.add, `has_one.one, `nat.add, `one],
   trace_state,
   t ← target,
   expected ← to_expr ```(a = succ b),
